

1. Use a limit definition of the derivative to find the derivative of the function $f(x) = \frac{1}{x+1}$.

$$\begin{aligned}
 f'(x) &= \lim_{z \rightarrow x} \frac{f(z) - f(x)}{z - x} = \lim_{z \rightarrow x} \frac{\frac{1}{z+1} - \frac{1}{x+1}}{z - x} \\
 &= \lim_{z \rightarrow x} \frac{\frac{1}{z+1} - \frac{1}{x+1}}{z - x} \cdot \frac{(z+1)(x+1)}{(z+1)(x+1)} \\
 &= \lim_{z \rightarrow x} \frac{(x+1) - (z+1)}{(z-x)(z+1)(x+1)} = \lim_{z \rightarrow x} \frac{-(z-x)}{(z-x)(z+1)(x+1)} \\
 &= \lim_{z \rightarrow x} \frac{-1}{(z+1)(x+1)} = \frac{-1}{(x+1)(x+1)} = \frac{-1}{(x+1)^2}
 \end{aligned}$$

Therefore: $f'(x) = \frac{-1}{(x+1)^2}$

Alternatively:

$$\begin{aligned}
 f'(x) &= \lim_{h \rightarrow 0} \frac{f(x+h) - f(x)}{h} = \lim_{h \rightarrow 0} \frac{\frac{1}{x+h+1} - \frac{1}{x+1}}{h} \\
 &= \lim_{h \rightarrow 0} \frac{\frac{1}{x+h+1} - \frac{1}{x+1}}{h} \cdot \frac{(x+h+1)(x+1)}{(x+h+1)(x+1)} \\
 &= \lim_{h \rightarrow 0} \frac{(x+1) - (x+h+1)}{h(x+h+1)(x+1)} = \lim_{h \rightarrow 0} \frac{-h}{h(x+h+1)(x+1)} \\
 &= \lim_{h \rightarrow 0} \frac{-1}{(x+h+1)(x+1)} = \frac{-1}{(x+0+1)(x+1)} = \frac{-1}{(x+1)^2}
 \end{aligned}$$

Therefore: $f'(x) = \frac{-1}{(x+1)^2}$

1. Use a limit definition of the derivative to find the derivative of the function $f(x) = \sqrt{x+1}$.

$$\begin{aligned}
 f'(x) &= \lim_{z \rightarrow x} \frac{f(z) - f(x)}{z - x} = \lim_{z \rightarrow x} \frac{\sqrt{z+1} - \sqrt{x+1}}{z - x} \\
 &= \lim_{z \rightarrow x} \frac{\sqrt{z+1} - \sqrt{x+1}}{z - x} \cdot \frac{\sqrt{z+1} + \sqrt{x+1}}{\sqrt{z+1} + \sqrt{x+1}} \\
 &= \lim_{z \rightarrow x} \frac{\sqrt{z+1}^2 + \sqrt{z+1}\sqrt{x+1} - \sqrt{x+1}\sqrt{z+1} - \sqrt{x+1}^2}{(z - x)(\sqrt{z+1} + \sqrt{x+1})} \\
 &= \lim_{z \rightarrow x} \frac{z+1 - (x+1)}{(z - x)(\sqrt{z+1} + \sqrt{x+1})} = \lim_{z \rightarrow x} \frac{(z - x)}{(z - x)(\sqrt{z+1} + \sqrt{x+1})} \\
 &= \lim_{z \rightarrow x} \frac{1}{\sqrt{z+1} + \sqrt{x+1}} = \frac{1}{\sqrt{x+1} + \sqrt{x+1}} = \frac{1}{2\sqrt{x+1}}
 \end{aligned}$$

Therefore: $f'(x) = \frac{1}{2\sqrt{x+1}}$

Alternatively:

$$\begin{aligned}
 f'(x) &= \lim_{h \rightarrow 0} \frac{f(x+h) - f(x)}{h} = \lim_{h \rightarrow 0} \frac{\sqrt{x+h+1} - \sqrt{x+1}}{h} \\
 &= \lim_{h \rightarrow 0} \frac{\sqrt{x+h+1} - \sqrt{x+1}}{h} \cdot \frac{\sqrt{x+h+1} + \sqrt{x+1}}{\sqrt{x+h+1} + \sqrt{x+1}} \\
 &= \lim_{h \rightarrow 0} \frac{(x+h+1) - (x+1)}{h(\sqrt{x+h+1} + \sqrt{x+1})} = \lim_{h \rightarrow 0} \frac{h}{h(\sqrt{x+h+1} + \sqrt{x+1})} \\
 &= \lim_{h \rightarrow 0} \frac{1}{\sqrt{x+h+1} + \sqrt{x+1}} = \frac{1}{\sqrt{x+0+1} + \sqrt{x+1}} = \boxed{\frac{1}{2\sqrt{x+1}}}
 \end{aligned}$$